feat: updateListWith

fstar/Zen.Sha3.Extracted.fst
@@ -6,8 +6,18 @@ open Zen.Cost
 module Sha3 = Zen.Sha3.Realized
 module PK = Zen.PublicKey
 
-val updateCPK : PK.cpk -> Sha3.t -> Sha3.t `cost` 203
+val updateCPK: PK.cpk -> Sha3.t -> Sha3.t `cost` 205
 let updateCPK (parity, h) s =
-    Sha3.updateByte parity s
-    >>= Sha3.updateHash h
-    |> Zen.Cost.inc 5
+  ret s
+  >>= Sha3.updateByte parity
+  >>= Sha3.updateHash h
+  |> Zen.Cost.inc 7
+
+val updateListWith (#a : Type) (#n : nat) :
+    (a -> Sha3.t -> Sha3.t `cost` n)
+    -> ls: list a
+    -> Sha3.t
+    -> Sha3.t `cost` (length ls * (n + 4) + 8)
+let rec updateListWith #_ #_ upd ls sha3 =
+  Zen.List.foldT (flip upd) sha3 ls
+  |> Zen.Cost.inc 4
